Printing flag for printing annotated boxes. Added simple erasure for types. Validation if constants and constructors are sufficiently applied. Deboxing of applications of global constants and constructors

erasure/theories/Debox.v
@@ -1,34 +1,592 @@
-From MetaCoq Require Import utils.
-From MetaCoq.Erasure Require Import EAst.
+From Coq Require Import Bool String Program List.
+From MetaCoq.Template Require Import config monad_utils utils uGraph Pretty All.
+From MetaCoq.PCUIC Require Import PCUICAst PCUICAstUtils PCUICTyping
+     TemplateToPCUIC PCUICInversion.
+From MetaCoq.SafeChecker Require Import PCUICSafeReduce PCUICSafeChecker
+     SafeTemplateChecker.
+From MetaCoq.Erasure Require ErasureFunction EAstUtils.
+From MetaCoq.Erasure Require Import SafeErasureFunction SafeTemplateErasure.
+
+Module EF := ErasureFunction.
+Module E := EAst.
+Module EUtils := EAstUtils.
+
+Import ListNotations.
+Import MonadNotation.
+
+Existing Instance envcheck_monad.
+Existing Instance extraction_checker_flags.
+
+Local Open Scope string_scope.
+
+Inductive box_type :=
+| TBox (_ : E.erasure_reason)
+| TArr (dom : box_type) (codom : box_type)
+| TApp (_ : box_type) (_ : box_type)
+| TRel (_ : nat)
+| TInd (_ : ident)
+| TConst (_ : ident).
+
+Fixpoint print_box_type  (bt : box_type) :=
+  match bt with
+  | TBox x => "⧈"
+  | TArr dom codom => print_box_type dom ++ " → " ++ print_box_type codom
+  | TApp t1 t2 => parens false (print_box_type t1 ++ " " ++ print_box_type t2)
+  | TRel i => "'a" ++ string_of_nat i
+  | TInd s => s
+  | TConst s => s
+  end.
+
+Ltac sq' := repeat match goal with
+         | H : ∥ _ ∥ |- _ => destruct H; try clear H
+         end; try eapply sq.
+
+Import PCUICSafeLemmata.
+
+
+Module P := PCUICAst.
+Module PInv := MetaCoq.PCUIC.PCUICInversion.
+
+Import PInv.
+
+Ltac solve_erase :=
+    sq;
+    let X := fresh "X" in
+    match goal with
+    | [H : welltyped _ _ (P.tEvar _ _) |- _ ] =>
+      destruct H as [? X];
+      (* inversion on evar gives [False] *)
+      now eapply inversion_Evar in X
+    | [H : welltyped _ _ (P.tLambda _ _ _) |- _  ] =>
+      destruct H as [? X];
+      eapply inversion_Lambda in X as (? & ? & ? & ? & ?);auto;eexists;eauto
+    | [H : welltyped _ _ (P.tLetIn _ _ _ _) |- _ ] =>
+      destruct H as [? X];
+      eapply inversion_LetIn in X as (? & ? & ? & ? & ? & ?);auto;eexists;eauto
+    | [H : welltyped _ _ (P.tApp _ _) |- _ ] =>
+      destruct H as [? X];
+      eapply inversion_App in X as (? & ? & ? & ? & ? & ?);auto;eexists;eauto
+    | [H : welltyped _ _ (P.tCase _ _ _ _) |- _] =>
+      destruct H as [? X];
+      eapply inversion_Case in X as
+          (? & ? & ? & ? & ? & ? & ? & ? & ? & ? & ? & ? & ? & ? & ?);auto;eexists;eauto
+    | [H : welltyped _ _ (P.tProj _ _)  |- _] =>
+      destruct H as [? X];
+      eapply inversion_Proj in X as
+          (? & ? & ? & ? & ? & ? & ? & ? & ?);auto;eexists;eauto
+    |  [H : welltyped _ _ (P.tProd _ _ _)  |- _] =>
+       destruct H as [? X];
+       eapply PInv.inversion_Prod in X as (? & ? & ? & ? & ?);auto;eexists;eauto
+    | [H : welltyped _ _ _  |- _] => destruct H as [? X];eexists;eauto
+    end.
+
+Program Fixpoint erase_type (Σ : P.global_env_ext)
+           (HΣ : ∥ PCUICTyping.wf_ext Σ ∥)
+           (Γ : PCUICAst.context)
+           (ty : P.term)
+           (* TODO: we need to pass [isType] instead, but this require to
+             implement the function in a different way *)
+           (Hty : welltyped Σ Γ ty)
+  : typing_result box_type :=
+  match (flag_of_type Σ HΣ Γ ty Hty) with
+  | Checked (Some r) => ret (TBox r)
+  | TypeError (NotASort _) (* TODO: figure out how to get rid of this case*)
+  | Checked None =>
+    match ty with
+    | P.tRel i => ret (TRel i)
+    | P.tSort _ => ret (TBox E.ER_type)
+    | P.tProd na b t =>
+      match flag_of_type Σ HΣ (P.vass na b :: Γ) t _  with
+          | Checked (Some _) => ret (TBox E.ER_type)
+          | Checked None =>
+            t1 <- erase_type Σ HΣ Γ b _ ;;
+            t2 <- erase_type Σ HΣ (P.vass na b :: Γ) t _ ;;
+            ret (TArr t1 t2)
+          | TypeError te => TypeError te
+      end
+    | P.tApp t1 t2 =>
+      t1' <- erase_type Σ HΣ Γ t1 _ ;;
+      t2' <- erase_type Σ HΣ Γ t2 _ ;;
+      ret (TApp t1' t2')
+    | P.tInd ind _ => ret (TInd ind.(inductive_mind))
+    | P.tLambda na t b => (* NOTE: assume that this is a type scheme, meaning that applied to enough args it ends up a type *)
+      erase_type Σ HΣ (P.vass na t :: Γ) b _
+    | P.tConst nm _ =>
+      (* NOTE: since the original term is well-typed, we know that the constant, applied to enough argument is a valid type (meaning that the constant is a type scheme), so, we just leave the constant name in the erased version *)
+      ret (TConst nm)
+    | P.tEvar _ _  | P.tCase _ _ _ _ | P.tProj _ _
+    | P.tFix _ _ | P.tCoFix _ _ | P.tVar _ | P.tLetIn _ _ _ _
+    | P.tConstruct _ _ _ => TypeError (Msg ("Not supported type: " ++ string_of_term ty))
+    end
+  | TypeError te => TypeError te
+  end.
+Solve Obligations with
+    (intros;
+    try (subst;
+        try clear dependent filtered_var;
+        try clear dependent filtered_var0;
+        try clear dependent Heq_anonymous;
+        try clear dependent Heq_anonymous0;solve_erase);try easy).
+
+
+Fixpoint mk_arrs (l : list box_type) (codom : box_type) :=
+  match l with
+  | [] => codom
+  | x :: l' => TArr x (mk_arrs l' codom)
+  end.
+
+Fixpoint mk_arrsM (l : (list (typing_result box_type))) (codom : box_type) :=
+  match l with
+  | [] => ret codom
+  | x :: l' =>
+    x' <- x ;;
+    res <- mk_arrsM l' codom ;;
+    ret (TArr x' res)
+  end.
+
+(* An attempt to reimplement erasure for types that always applied to a well-formed types. This breaks when we do a recurison in the application case.
+  Using decompose_app requires some well-foundness argument for fix *)
+
+(* Program Fixpoint erase_type (Σ : P.global_env_ext) *)
+(*            (HΣ : ∥ PCUICTyping.wf_ext Σ ∥) *)
+(*            (Γ : PCUICAst.context) *)
+(*            (ty : P.term) *)
+(*            (Hty :  ∥ isType Σ Γ ty ∥) *)
+(*   : typing_result box_type := *)
+(*   match (flag_of_type Σ HΣ Γ ty _) with *)
+(*   | Checked (Some r) => ret (TBox r) *)
+(*   | TypeError (NotASort _) | Checked None => *)
+(*     match ty with *)
+(*     | P.tRel i => ret (TRel i) *)
+(*     | P.tSort _ => ret (TBox E.ER_type) *)
+(*     | P.tProd na b t => *)
+(*       match flag_of_type Σ HΣ (P.vass na b :: Γ) t _  with *)
+(*           | Checked (Some _) => ret (TBox E.ER_type) *)
+(*           | Checked None => *)
+(*             t1 <- erase_type Σ HΣ Γ b _ ;; *)
+(*             t2 <- erase_type Σ HΣ (P.vass na b :: Γ) t _ ;; *)
+(*             ret (TArr t1 t2) *)
+(*           | TypeError te => TypeError te *)
+(*       end *)
+(*     | P.tApp t1 t2 => *)
+(*       let '(t, args) := decompose_app t1 in *)
+(*       let eargs := map (fun x => erase_type Σ HΣ Γ x _) args in *)
+(*       t2' <- erase_type Σ HΣ Γ t2 _ ;; *)
+(*       (* t2' <- erase_type Σ HΣ Γ t2 _ ;; *) *)
+(*       res <- mk_arrsM eargs t2' ;; *)
+(*       (* ret (TApp (TInd "") t2') *) *)
+(*       ret (TApp (TInd "") t2') *)
+(*     | P.tInd ind _ => ret (TInd ind.(inductive_mind)) *)
+(*     | P.tLambda na t b => (* NOTE: assume that this is a type scheme, meaning that applied to enough args it ends up a type *) *)
+(*       erase_type Σ HΣ (P.vass na t :: Γ) b _ *)
+(*     | P.tConst nm _ => *)
+(*       (* NOTE: since the original term is well-typed, we know that the constant, applied to enough argument is a valid type (meaning that the constant is a type scheme), so, we just leave the constant name in the erased version *) *)
+(*       ret (TConst nm) *)
+(*     | P.tEvar _ _  | P.tCase _ _ _ _ | P.tProj _ _ *)
+(*     | P.tFix _ _ | P.tCoFix _ _ | P.tVar _ | P.tLetIn _ _ _ _ *)
+(*     | P.tConstruct _ _ _ => TypeError (Msg ("Not supported type: " ++ string_of_term ty)) *)
+(*     end *)
+(*   | TypeError te => TypeError te *)
+(*   end. *)
+(* Solve Obligations with *)
+(*     (intros; *)
+(*     try (subst; *)
+(*         try clear dependent filtered_var; *)
+(*         try clear dependent filtered_var0; *)
+(*         try clear dependent Heq_anonymous; *)
+(*         try clear dependent Heq_anonymous0;solve_erase);try easy). *)
+(* Next Obligation. *)
+(*   try clear dependent Heq_anonymous0. *)
+(*   sq. destruct Hty as [? X]. *)
+(*   eapply inversion_App in X as (? & ? & ? & ? & ? & ?);auto. *)
+(*   ;eexists;eauto. *)
+(*   eexists;eauto. *)
+(* Qed. *)
+(* Next Obligation. *)
+(*   try clear dependent Heq_anonymous; *)
+(*     try clear dependent Heq_anonymous0. *)
+(*   (* destruct Hty as [? X]. *) *)
+(*   solve_erase. *)
+(*   sq;match goal with *)
+(*     |  [H : isType _ _ (P.tProd _ _ _)  |- _] => *)
+(*        destruct H as [? X]; *)
+(*          eapply PInv.inversion_Prod in X as (? & ? & ? & ? & ?);auto;eexists;eauto *)
+(*   end. *)
+(*   solve_erase. *)
+(*   eapply PInv.inversion_Prod in X as (? & ? & ? & ? & ?);auto;eexists;eauto. *)
+(* Qed. *)
+
+Program Definition erase_type_program (p : Ast.program)
+  : EnvCheck (EAst.global_context * box_type) :=
+  let Σ := List.rev (trans_global (Ast.empty_ext p.1)).1 in
+  G <- check_wf_env_only_univs Σ ;;
+  Σ' <- wrap_error (empty_ext Σ) "erasure of the global context" (SafeErasureFunction.erase_global Σ _) ;;
+  t <- wrap_error (empty_ext Σ) ("During erasure of " ++ string_of_term (trans p.2)) (erase_type (empty_ext Σ) _ nil (trans p.2) _);;
+  ret (Monad:=envcheck_monad) (Σ', t).
+Next Obligation.
+  unfold trans_global.
+  simpl. unfold wf_ext, empty_ext. simpl.
+  unfold on_global_env_ext. destruct H0. constructor.
+  split; auto. simpl. todo "on_udecl on empty universe context".
+Qed.
+
+Next Obligation.
+  unfold trans_global.
+  simpl. unfold wf_ext, empty_ext. simpl.
+  unfold on_global_env_ext. destruct H0. todo "assuming well-typedness".
+Qed.
+
+Definition erase_and_print_type {cf : checker_flags} (p : Ast.program)
+  : string + string :=
+  let p := fix_program_universes p in
+  match erase_type_program p return string + string with
+  | CorrectDecl (Σ', t) =>
+    inl ("Environment is well-formed and " ++ Pretty.print_term (Ast.empty_ext p.1) [] true p.2 ++
+         " erases to: " ++ nl ++ print_box_type t)
+  | EnvError Σ' (AlreadyDeclared id) =>
+    inr ("Already declared: " ++ id)
+  | EnvError Σ' (IllFormedDecl id e) =>
+    inr ("Type error: " ++ PCUICSafeChecker.string_of_type_error Σ' e ++ ", while checking " ++ id)
+  end.
+
+
+Quote Recursively Definition ex1 := (forall (A : Type),  list A -> 0 = 0 -> A).
+Compute erase_and_print_type ex1.
+
+Definition non_neg := {n : nat | 0 < n}.
+
+Quote Recursively Definition ex2 := (forall (A : Type), {n : nat | 0 < n} -> A).
+Compute erase_and_print_type ex2.
+
+Fixpoint lookup_env (Σ : P.global_env) (id : ident) : option P.global_decl :=
+  match Σ with
+  | nil => None
+  | hd :: tl =>
+    if ident_eq id hd.1 then Some hd.2
+    else lookup_env tl id
+  end.
+
+Definition lookup_ind_decl (Σ : P.global_env) ind i :=
+  match lookup_env Σ ind with
+  | Some (P.InductiveDecl {| P.ind_bodies := l; P.ind_universes := uctx |}) =>
+    match nth_error l i with
+    | Some body => Some body
+    | None => None
+    end
+  | _ => None
+  end.
+
+Definition lookup_const (Σ : P.global_env) const :=
+  match lookup_env Σ const with
+  | Some (P.ConstantDecl b) => Some b
+  | _ => None
+  end.
 
 Definition get_shift (n : nat) (g : list bool) :=
   List.count_occ Bool.bool_dec (List.firstn (1+n) g) true.
 
-Fixpoint debox (g : list bool) (t : term) :=
+Fixpoint debox_types (g : list bool) (t : E.term) :=
   match t with
-  | tRel i => tRel (i - get_shift i g)
-  | tEvar ev args => tEvar ev (List.map (debox g) args)
-  | tLambda na M => match na.(binder_erasure_reason) with
-                   | Some ER_type => debox (true :: g) M
-                   | _ => tLambda na (debox (false :: g) M)
+  | E.tRel i => E.tRel (i - get_shift i g)
+  | E.tEvar ev args => E.tEvar ev (List.map (debox_types g) args)
+  | E.tLambda na M => match na.(E.binder_erasure_reason) with
+                   | Some ER_type => debox_types (true :: g) M
+                   | _ => E.tLambda na (debox_types (false :: g) M)
                    end
-  | tApp u v => match v with
-               | tBox ER_type => debox g u
-               | _ => tApp (debox g u) (debox g v)
+  | E.tApp u v => match v with
+               | E.tBox ER_type => debox_types g u
+               | _ => E.tApp (debox_types g u) (debox_types g v)
                end
-  | tLetIn na b b' => tLetIn na (debox g b) (debox (false :: g) b')
-  | tCase ind c brs =>
-    let brs' := List.map (on_snd (debox g)) brs in
-    tCase ind (debox g c) brs'
-  | tProj p c => tProj p (debox g c)
-  | tFix mfix idx =>
-    let mfix' := List.map (map_def (debox g)) mfix in
-    tFix mfix' idx
-  | tCoFix mfix idx =>
-    let comfix' := List.map (map_def (debox g)) mfix in
-    tCoFix comfix' idx
-  | tBox r => t
-  | tVar _ => t
-  | tConst _ => t
-  | tConstruct _ _ => t
+  | E.tLetIn na b b' => E.tLetIn na (debox_types g b) (debox_types (false :: g) b')
+  | E.tCase ind c brs =>
+    let brs' := List.map (on_snd (debox_types g)) brs in
+    E.tCase ind (debox_types g c) brs'
+  | E.tProj p c => E.tProj p (debox_types g c)
+  | E.tFix mfix idx =>
+    let mfix' := List.map (E.map_def (debox_types g)) mfix in
+    E.tFix mfix' idx
+  | E.tCoFix mfix idx =>
+    let comfix' := List.map (E.map_def (debox_types g)) mfix in
+    E.tCoFix comfix' idx
+  | E.tBox r => t
+  | E.tVar _ => t
+  | E.tConst _ => t
+  | E.tConstruct _ _ => t
   end.
+
+(* TODO : should go to the EAstUtils module *)
+Fixpoint isConstruct_app (t : E.term) : bool :=
+  match (EUtils.decompose_app t).1 with
+  | E.tConstruct _ _  => true
+  | _ => false
+  end.
+
+(* TODO : should go to the EAstUtils module *)
+Fixpoint isConst_app (t : E.term) : bool :=
+  match (EUtils.decompose_app t).1 with
+  | E.tConst _ => true
+  | _ => false
+  end.
+
+
+SearchPattern (term -> bool).
+About isConst_app.
+
+(** Remove all boxes applied to global constants and contructors.
+    Assumes that constants applied to all logical arguments and constructors are fylly applied. *)
+Fixpoint debox_all (t : E.term) :=
+  match t with
+  | E.tRel i => E.tRel i
+  | E.tEvar ev args => E.tEvar ev (List.map debox_all args)
+  | E.tLambda na M => E.tLambda na (debox_all M)
+  | E.tApp u v =>
+    match v with
+    | E.tBox _ =>
+      if (isConstruct_app u || isConst_app u)
+      then debox_all u (* ignore the box if it's applied to a constructor or a global constant*)
+      else E.tApp (debox_all u) (debox_all v)
+    | _ => E.tApp (debox_all u) (debox_all v)
+    end
+  | E.tLetIn na b b' => E.tLetIn na (debox_all b) (debox_all b')
+  | E.tCase ind c brs =>
+    let brs' := List.map (on_snd debox_all) brs in
+    E.tCase ind (debox_all c) brs'
+  | E.tProj p c => E.tProj p (debox_all c)
+  | E.tFix mfix idx =>
+    let mfix' := List.map (E.map_def debox_all) mfix in
+    E.tFix mfix' idx
+  | E.tCoFix mfix idx =>
+    let comfix' := List.map (E.map_def debox_all) mfix in
+    E.tCoFix comfix' idx
+  | E.tBox r => t
+  | E.tVar _ => t
+  | E.tConst _ => t
+  | E.tConstruct _ _ => t
+  end.
+
+
+Fixpoint adjust_indices (g : list bool) (t : E.term) :=
+  match t with
+  | E.tRel i => E.tRel (i - get_shift i g)
+  | E.tEvar ev args => E.tEvar ev (List.map (adjust_indices g) args)
+  | E.tLambda na M =>
+    (* we always push [false], bacuse we only adjust for top-level lambdas *)
+    E.tLambda na (adjust_indices (false :: g) M)
+  | E.tApp u v => E.tApp (adjust_indices g u) (adjust_indices g v)
+  | E.tLetIn na b b' =>
+    (* we always push [false], bacuse we only adjust for top-level lambdas *)
+    E.tLetIn na (adjust_indices g b) (adjust_indices (false :: g) b')
+  | E.tCase ind c brs =>
+    let brs' := List.map (on_snd (adjust_indices g)) brs in
+    E.tCase ind (adjust_indices g c) brs'
+  | E.tProj p c => E.tProj p (adjust_indices g c)
+  | E.tFix mfix idx =>
+    let mfix' := List.map (E.map_def (adjust_indices g)) mfix in
+    E.tFix mfix' idx
+  | E.tCoFix mfix idx =>
+    let comfix' := List.map (E.map_def (adjust_indices g)) mfix in
+    E.tCoFix comfix' idx
+  | E.tBox r => t
+  | E.tVar _ => t
+  | E.tConst _ => t
+  | E.tConstruct _ _ => t
+  end.
+
+Fixpoint decompose_arr (t : box_type) : list box_type × box_type :=
+  match t with
+  | TArr A B =>
+      let (dom, codom) := decompose_arr B in
+      (A :: dom, codom)
+  | _ => ([], t)
+  end.
+
+
+Definition keep (o : option E.erasure_reason) : bool :=
+  match o with
+  | Some _ => false
+  | None   => true
+  end.
+
+Definition is_TBox (ty : box_type) :=
+  match ty with
+  | TBox x => true
+  | _ => false
+  end.
+
+Fixpoint Edecompose_lam (t : E.term) : (list E.aname) × E.term :=
+  match t with
+  | E.tLambda n b =>
+      let (ns, b) := Edecompose_lam b in
+      (n :: ns, b)
+  | _ => ([], t)
+  end.
+
+Definition Eit_mkLambda (l : list E.aname) (t : E.term) :=
+fold_left (fun acc nm => E.tLambda nm acc) l t.
+
+Definition debox_top_level (t : E.term) :=
+  let (params, body) := Edecompose_lam t in
+  let bitmask := rev (map (negb ∘ keep ∘ E.binder_erasure_reason) params) in
+  let filtered_params := rev (filter (keep ∘ E.binder_erasure_reason) params) in
+  Eit_mkLambda filtered_params (adjust_indices bitmask body).
+
+Section DeboxTopLevelExamples.
+  Definition x := E.mkBindAnn (nNamed "x") None.
+  Definition y := E.mkBindAnn (nNamed "y") None.
+  Definition p := E.mkBindAnn (nNamed "x") (Some E.ER_prop).
+  Example debox_top_level_1 :
+    debox_top_level
+      (E.tLambda x (E.tLambda p (E.tLambda y (E.tApp (E.tRel 2) (E.tRel 0))))) =
+    (E.tLambda x (E.tLambda y (E.tApp (E.tRel 1) (E.tRel 0)))).
+  Proof. reflexivity. Qed.
+
+  Example debox_top_level_2 :
+    debox_top_level
+      (E.tLambda x (E.tLambda y (E.tLambda p (E.tApp (E.tRel 2) (E.tRel 1))))) =
+    (E.tLambda x (E.tLambda y (E.tApp (E.tRel 1) (E.tRel 0)))).
+  Proof. reflexivity. Qed.
+End DeboxTopLevelExamples.
+
+Definition is_fully_applied_ctor (Σ : P.global_env)
+           (ind : inductive)
+           (ctor : nat) (n_app : nat) :=
+  match PCUICChecker.lookup_constructor_decl Σ ind.(inductive_mind) ind.(inductive_ind) ctor with
+  | PCUICChecker.Checked (_,_,ty) =>
+    let (dom, _) :=
+        PCUICAstUtils.decompose_prod ty in
+    Nat.eqb n_app (length dom.2)
+  | _ => false
+  end.
+
+Definition find_indices {A : Type}
+           (f : A -> bool) : list A -> list nat :=
+  let worker := fix go (i : nat) l :=
+              match l with
+              | [] => []
+              | x :: tl =>
+                if f x then i :: go (1+i)%nat tl
+                else go (1+i)%nat tl
+              end in
+  worker 0.
+
+Fixpoint last_option {A} (l : list A) : option A :=
+  match l with
+  | [] => None
+  | [a] => Some a
+  | a :: (_ :: _) as l0 => last_option l0
+  end.
+
+Definition last_box_index l := last_option (find_indices is_TBox l).
+
+Compute last_box_index
+        (decompose_arr (TArr (TBox (E.ER_type))
+                       ((TArr (TRel 0) (TArr (TBox (E.ER_type)) (TRel 1)))))).1.
+
+Program Definition is_logargs_applied_const (Σ : P.global_env_ext)
+           (HΣ : ∥ PCUICTyping.wf_ext Σ ∥)
+           (Γ : PCUICAst.context)
+           (const : ident) (n_app : nat) : typing_result bool :=
+  match lookup_const Σ const with
+  | Some b =>
+    ety <- erase_type Σ HΣ Γ b.(P.cst_type) _ ;;
+    let (dom, _) := decompose_arr ety in
+    match last_box_index dom with
+    | Some i => ret (Nat.leb (i+1) n_app)
+    | None => ret true
+    end
+  | _ => TypeError (Msg ("Constant not found: " ++ const))
+  end.
+Next Obligation.
+  sq. destruct Σ; destruct HΣ as [p1 p2];simpl in *.
+  todo "everything coming from well-formed environment is well typed".
+Qed.
+
+Program Definition test_applied_to_logargs  (p : Ast.program) (const : ident) (n_app : nat)
+  : EnvCheck bool :=
+  let p := fix_program_universes p in
+  let Σ := List.rev (trans_global (Ast.empty_ext p.1)).1 in
+  G <- check_wf_env_only_univs Σ ;;
+  t <- wrap_error (empty_ext Σ) "during cheking applied constant" (is_logargs_applied_const (empty_ext Σ) _ [] const n_app) ;;
+  ret (Monad:=envcheck_monad) t.
+Next Obligation.
+  unfold trans_global.
+  simpl. unfold wf_ext, empty_ext. simpl.
+  unfold on_global_env_ext. destruct H0. constructor.
+  split; auto. simpl. todo "on_udecl on empty universe context".
+Qed.
+
+Quote Recursively Definition ex3 := combine.
+
+Compute (test_applied_to_logargs ex3 "Coq.Lists.List.combine" 2).
+
+Definition test_fully_applied_constructor (p : Ast.program) (ind_nm : ident) (ind_i : nat) (ctor : nat) (n_app : nat) :=
+  let p := fix_program_universes p in
+  let Σ := List.rev (trans_global (Ast.empty_ext p.1)).1 in
+  (is_fully_applied_ctor Σ (mkInd ind_nm ind_i) ctor n_app).
+
+Quote Recursively Definition q_prod
+  := (fun (x y : nat) => (x,y)).
+
+Compute ((test_fully_applied_constructor q_prod "Coq.Init.Datatypes.prod" 0 0 4)).
+
+
+Definition forallb_defs {A : Set} (f : A -> bool) (ds : list (E.def A)) :=
+  (* this way of defining is fixpoint-firendly, i.e. is we [map] first and then apply [forallb] it fails to work with the definition below *)
+  forallb (fun x => f x.(E.dbody)) ds.
+
+Definition check_ctors_applied (Σ : P.global_env) :=
+  fix go (apps : list E.term) (t : E.term) :=
+    match t with
+    | E.tRel i => true
+    | E.tEvar ev args => forallb (go []) args
+    | E.tLambda na M => go [] M
+    | E.tApp u v => (go (v :: apps) u) && (go [] v)
+    | E.tLetIn na b b' => (go [] b) && (go [] b')
+    | E.tCase ind c brs =>
+      let brs' := forallb (fun x => go [] (snd x)) brs in
+      (go [] c) && brs'
+    | E.tProj p c => go [] c
+    | E.tFix mfix idx =>
+      forallb_defs (go []) mfix
+    | E.tCoFix mfix idx =>
+      forallb_defs (go []) mfix
+    | E.tBox r => true
+    | E.tVar _ => true
+    | E.tConst _ => true
+    | E.tConstruct ind i =>
+      is_fully_applied_ctor Σ ind i (length apps)
+    end.
+
+Definition check_consts_applied
+  (Σ : P.global_env_ext) (HΣ : ∥ PCUICTyping.wf_ext Σ ∥) :=
+  fix go (apps : list E.term) (t : E.term) : typing_result bool:=
+    match t with
+    | E.tRel i => ret true
+    | E.tEvar ev args =>
+      res <- monad_map (go []) args ;;
+      ret (forallb id res)
+    | E.tLambda na M => go [] M
+    | E.tApp u v =>
+      b1 <- go (v :: apps) u ;;
+      b2 <- go [] v ;;
+      ret (b1 && b2)
+    | E.tLetIn na b b' =>
+      b1 <- go [] b;;
+      b2 <- go [] b';;
+      ret (b1 && b2)
+    | E.tCase ind c brs =>
+      b1 <- go [] c ;;
+      res <- monad_map (fun x => go [] (snd x)) brs ;;
+      ret (b1 && forallb id res)
+    | E.tProj p c => go [] c
+    | E.tFix mfix idx =>
+      res <- monad_map (fun x => go [] (E.dbody x)) mfix ;;
+      ret (forallb id res)
+    | E.tCoFix mfix idx =>
+      res <- monad_map (fun x => go [] (E.dbody x)) mfix ;;
+      ret (forallb id res)
+    | E.tBox r => ret true
+    | E.tVar _ => ret true
+    | E.tConst nm => is_logargs_applied_const Σ HΣ [] nm (length apps)
+    | E.tConstruct ind i => ret true
+    end.
